isabelle/core/CoreTypeProps.thy
@@ -135,9 +135,9 @@ lemma is_runtime_type_cong_env:
    is_runtime_type env' ty = is_runtime_type env ty"
   by (induction ty) (auto simp: list_all_iff)
 
-lemma is_runtime_type_TE_ConstNames_irrelevant [simp]:
-  "is_runtime_type (env \<lparr> TE_ConstNames := c \<rparr>) ty = is_runtime_type env ty"
-  using is_runtime_type_cong_env[of "env \<lparr> TE_ConstNames := c \<rparr>" env] by simp
+lemma is_runtime_type_TE_ConstLocals_irrelevant [simp]:
+  "is_runtime_type (env \<lparr> TE_ConstLocals := c \<rparr>) ty = is_runtime_type env ty"
+  using is_runtime_type_cong_env[of "env \<lparr> TE_ConstLocals := c \<rparr>" env] by simp
 
 (* If ty is runtime in an env, then every type variable in ty is in the env's
    TE_RuntimeTypeVars. *)
