isabelle/interpreter/CoreInterpPreservation.thy
@@ -40,7 +40,7 @@ proof -
       have state'_eq:
         "state' = (fst ?alloc) \<lparr> IS_Locals := fmupd name (snd ?alloc) (IS_Locals (fst ?alloc)),
                                   IS_Refs := fmdrop name (IS_Refs (fst ?alloc)),
-                                  IS_ConstNames := finsert name (IS_ConstNames (fst ?alloc)) \<rparr>"
+                                  IS_ConstLocals := finsert name (IS_ConstLocals (fst ?alloc)) \<rparr>"
         by (simp add: case_prod_beta)
       have "IS_Globals (fst ?alloc) = IS_Globals state"
            "IS_Functions (fst ?alloc) = IS_Functions state"
@@ -65,7 +65,7 @@ proof -
         from arg_eq Ref \<open>refRes = Inr addrPath\<close> addrPath_eq Inr assms
         have "state' = state \<lparr> IS_Locals := fmdrop name (IS_Locals state),
                                 IS_Refs := fmupd name (addr, path) (IS_Refs state),
-                                IS_ConstNames := fminus (IS_ConstNames state) {|name|} \<rparr>"
+                                IS_ConstLocals := fminus (IS_ConstLocals state) {|name|} \<rparr>"
           by simp
         then show ?thesis by simp
       qed
@@ -237,7 +237,7 @@ next
           with H CoreStmt_VarDecl have
             "res = Continue (state \<lparr> IS_Locals := fmdrop varName (IS_Locals state),
                                       IS_Refs := fmdrop varName (IS_Refs state),
-                                      IS_ConstNames := fminus (IS_ConstNames state) {|varName|} \<rparr>)"
+                                      IS_ConstLocals := fminus (IS_ConstLocals state) {|varName|} \<rparr>)"
             by simp
           then show ?thesis by (simp add: exec_result_preserves_gf_Continue)
         next
@@ -264,8 +264,8 @@ next
               have res_eq: "res = Continue ((fst ?alloc) \<lparr> IS_Locals :=
                                fmupd varName (snd ?alloc) (IS_Locals (fst ?alloc)),
                                IS_Refs := fmdrop varName (IS_Refs (fst ?alloc)),
-                               IS_ConstNames :=
-                                 fminus (IS_ConstNames (fst ?alloc)) {|varName|} \<rparr>)"
+                               IS_ConstLocals :=
+                                 fminus (IS_ConstLocals (fst ?alloc)) {|varName|} \<rparr>)"
                 by (simp add: case_prod_beta)
               have alloc_gf: "IS_Globals (fst ?alloc) = IS_Globals newState"
                              "IS_Functions (fst ?alloc) = IS_Functions newState"
@@ -282,8 +282,8 @@ next
               have res_eq: "res = Continue ((fst ?alloc) \<lparr> IS_Locals :=
                                fmupd varName (snd ?alloc) (IS_Locals (fst ?alloc)),
                                IS_Refs := fmdrop varName (IS_Refs (fst ?alloc)),
-                               IS_ConstNames :=
-                                 fminus (IS_ConstNames (fst ?alloc)) {|varName|} \<rparr>)"
+                               IS_ConstLocals :=
+                                 fminus (IS_ConstLocals (fst ?alloc)) {|varName|} \<rparr>)"
                 by (cases initTm; simp_all add: case_prod_beta)
               have "IS_Globals (fst ?alloc) = IS_Globals state"
                    "IS_Functions (fst ?alloc) = IS_Functions state"
@@ -298,7 +298,7 @@ next
               base: "lvalue_base_name initTm = Some baseName"
               by (cases "lvalue_base_name initTm") simp_all
             show ?thesis
-            proof (cases "baseName |\<in>| IS_ConstNames state
+            proof (cases "baseName |\<in>| IS_ConstLocals state
                           \<or> (fmlookup (IS_Locals state) baseName = None
                              \<and> fmlookup (IS_Refs state) baseName = None)")
               case True
@@ -312,8 +312,8 @@ next
                  ((fst ?alloc) \<lparr> IS_Locals :=
                                   fmupd varName (snd ?alloc) (IS_Locals (fst ?alloc)),
                                  IS_Refs := fmdrop varName (IS_Refs (fst ?alloc)),
-                                 IS_ConstNames :=
-                                  finsert varName (IS_ConstNames (fst ?alloc)) \<rparr>)"
+                                 IS_ConstLocals :=
+                                  finsert varName (IS_ConstLocals (fst ?alloc)) \<rparr>)"
                 by (simp add: case_prod_beta)
               have "IS_Globals (fst ?alloc) = IS_Globals state"
                    "IS_Functions (fst ?alloc) = IS_Functions state"
@@ -330,7 +330,7 @@ next
               have res_eq: "res = Continue
                  (state \<lparr> IS_Locals := fmdrop varName (IS_Locals state),
                           IS_Refs := fmupd varName addrPath (IS_Refs state),
-                          IS_ConstNames := fminus (IS_ConstNames state) {|varName|} \<rparr>)"
+                          IS_ConstLocals := fminus (IS_ConstLocals state) {|varName|} \<rparr>)"
                 by simp
               then show ?thesis by (simp add: exec_result_preserves_gf_Continue)
             qed
@@ -608,7 +608,7 @@ next
       let ?valResults = "map (interp_term fuel state) argTms"
       let ?argTuples = "zip (IF_Args f) (zip ?refResults ?valResults)"
       let ?clearedState = "state \<lparr> IS_Locals := fmempty, IS_Refs := fmempty,
-                                     IS_ConstNames := {||} \<rparr>"
+                                     IS_ConstLocals := {||} \<rparr>"
       have cleared_gf:
         "IS_Globals ?clearedState = IS_Globals state"
         "IS_Functions ?clearedState = IS_Functions state"
